Term.v
@@ -19,3 +19,26 @@ Inductive term : Set :=
   | Apply   : term  -> term -> term
   | If      : term -> term -> term -> term.
 
+Fixpoint term_length (t : term) :=
+  match t with
+  |  Var _ | Bool _ =>
+    1
+  | Lambda _ _ body =>
+    1 + term_length body
+  | Apply t1 t2 =>
+    1 + term_length t1 + term_length t2
+  | If t1 t2 t3 =>
+    1 + term_length t1 + term_length t2 + term_length t3
+  end.
+
+Inductive FV : string -> term -> Prop :=
+  | FVVar    : forall s, FV s (Var s)
+  | FVLambda : forall x y t T, x <> y -> FV x t -> FV x (Lambda y T t)
+  | FVApply  : forall x t1 t2, FV x t1 \/ FV x t2 -> FV x (Apply t1 t2)
+  | FVIf     : forall x t1 t2 t3, FV x t1 \/ FV x t2 \/ FV x t3 -> FV x (If t1 t2 t3).
+
+Inductive BV : string -> term -> Prop :=
+  | BVLambda1 : forall x T t, BV x (Lambda x T t)
+  | BVLambda2 : forall x y T t, BV x t -> BV x (Lambda y T t)
+  | BVApply   : forall x t1 t2, BV x t1 \/ BV x t2 -> BV x (Apply t1 t2)
+  | BVIf      : forall x t1 t2 t3, BV x t1 \/ BV x t2 \/ BV x t3 -> BV x (If t1 t2 t3).
