Alpha.v
@@ -1,0 +1,63 @@
+Require Import List.
+Require Import String.
+
+Require Import Term.
+
+Variable Flesh : string -> term -> term -> string.
+Hypothesis Flesh_x : forall x s t, x <> Flesh x s t.
+Hypothesis Flesh_fv1 : forall x s t, ~FV (Flesh x s t) s.
+Hypothesis Flesh_fv2 : forall x s t, ~FV (Flesh x s t) t.
+Hypothesis Flesh_bv : forall x s t, ~BV (Flesh x s t) t.
+
+Fixpoint alpha (t : term) (old new : string) :=
+  match t with
+  |  Var s =>
+    if string_dec s old then
+      Var new
+    else
+      t
+  | Bool _  =>
+      t
+  | Lambda x T body =>
+      if string_dec x old then
+      	Lambda x T body
+      else
+        Lambda x T (alpha body old new)
+  | Apply t1 t2 =>
+      Apply (alpha t1 old new) (alpha t2 old new)
+  | If t1 t2 t3 =>
+      If (alpha t1 old new) (alpha t2 old new) (alpha t3 old new)
+  end.
+
+Theorem alpha_length :
+  forall (t : term) (x y : string),
+  term_length t = term_length (alpha t x y).
+Proof.
+induction t.
+ simpl in |- *.
+ intros.
+ destruct string_dec; simpl in |- *; reflexivity.
+
+ simpl in |- *.
+ intros; reflexivity.
+
+ simpl in |- *.
+ intros.
+ destruct (string_dec s x); simpl in |- *.
+  reflexivity.
+
+  rewrite (IHt x y) in |- *.
+  reflexivity.
+
+ simpl in |- *.
+ intros.
+ rewrite (IHt1 x y) in |- *.
+ rewrite (IHt2 x y) in |- *.
+ reflexivity.
+
+ simpl in |- *.
+ intros.
+ rewrite (IHt1 x y) in |- *; rewrite (IHt2 x y) in |- *;
+  rewrite (IHt3 x y) in |- *.
+ reflexivity.
+Qed.
